
- $x,y \in R$
- $n \in N$

$$
(x+y)^n = \sum^n_{k=0} C^k_n x^k y^{n-k}
$$

- $(1+x)^n$ - Obyčejná vytvořující funkce koeficientů $\{C^k_n\}^\infty_0$


1. 2. ... n.
$(x+y)(x+y)...(x+y)$

$$
P(k,n-k) x^k y^{n-k}
= C^k_n x^k y^{n-k}
$$

jiný zápis:
$$
(1+x)^n = \sum^n_{k=0} \binom{n}{k} x^k
$$

$$
(1+x)^\alpha = \sum_{k=0}^{\infty} \binom{\alpha}{k} x^k
$$

- $\alpha \in R$

> [!tip]
> Také jako Taylorův rozvoj v bodě $0$.

$$
\binom{\alpha}{k} = \frac{\alpha (\alpha - 1) (\alpha - 2) ... (\alpha - k + 1)}{k!}
$$