# Newtonův vzorec
$x \in R$
$|x| < 1$
$\alpha \in R$

$$
(1+x)^\alpha = 
1 + \alpha x + \frac{\alpha(\alpha-1)}{2!}x^2 +...+
\frac{\alpha(\alpha-1)*...*(\alpha-k+1)}{k!}+...
$$
- Taylorův rozvoj

$n \in N$

$$
(1+x)^n = 
1 + n x + \frac{n(n-1)}{2!}x^2 +...+
\frac{n(n-1)*...*(n-k+1)}{k!}+...
$$


$$
\frac{n!}{k!(n-k)!} = C^k_n
$$
Newtonův vzorec přejde v binomický vzorec pro ...

$-n$

$$
(-1)^k 
\frac
{n(n+1)!*...*(n+k-1)}
{k!}
* \frac{(n-1)!}{(n-1)!}
$$
nějaký další hegeš...

$$
= (-1)^k C^k_{n+k-1}
$$